Save work in progress

boogie/red-black-tree/delete.bpl
@@ -6,3 +6,501 @@
 //
 // Verification of Red-Black Tree Delete.
 
+procedure RBTFindMinContract(x: Ref) returns (ret: int);
+    requires x != null;
+    requires RefSetsDisjoint(Br, C.repr[x]);
+    requires LC(C.k, C.l, C.r, C.p, 
+                C.min, C.max, C.keys,
+                C.repr, C.black, C.black_height, 
+                x);
+    ensures (C.keys[x])[ret];
+    ensures ret == C.min[x];
+
+procedure RBTDeleteLeftFixupContract(x: Ref) 
+    returns (ret: Ref, fixed: bool);
+    requires x != null;
+    requires RefSetsDisjoint(Br, (C.repr[x])[x := false]);
+    requires LC_Trans_DoubleBlack(C.k, C.l, C.r, C.p, 
+                C.min, C.max, C.keys,
+                C.repr, C.black, C.black_height, 
+                x);
+    requires (C.l[x] == null && C.r[x] != null && C.black_height[C.r[x]] == 1)
+            || (C.l[x] != null && C.r[x] != null && C.black_height[C.l[x]] + 1 == C.black_height[C.r[x]]);
+    requires (C.l[x] == null || C.black[C.l[x]]);
+    requires (C.black[x] || (C.r[x] == null || C.black[C.r[x]]));
+    modifies Br, C.k, C.l, C.r, C.p, 
+                C.min, C.max, C.keys,
+                C.repr, C.black, C.black_height;
+    ensures ret != null;
+    ensures x != ret ==> (
+        C.p[x] != null
+        && C.p[x] != old(C.p)[x]
+        && (C.repr[ret])[C.p[x]]
+        && (C.l[x] != null ==> (C.repr[ret])[C.l[x]])
+        && (C.r[x] != null ==> (C.repr[ret])[C.r[x]])
+    );
+    ensures LC(C.k, C.l, C.r, C.p, 
+                C.min, C.max, C.keys,
+                C.repr, C.black, C.black_height, 
+                ret);
+    ensures C.p[ret] == null;
+    ensures KeySetsEqual(C.keys[ret], old(C.keys)[x]);
+    ensures C.min[ret] == old(C.min)[x];
+    ensures C.max[ret] == old(C.max)[x];
+    ensures RefSetsEqual(C.repr[ret], old(C.repr)[x]);
+    ensures C.black[ret] || (!C.black[ret] && !old(C.black)[x]);
+    ensures (fixed && C.black_height[ret] == old(C.black_height)[x])
+            ||  (!fixed && old(C.black)[x] && C.black_height[ret] == old(C.black_height)[x] - 1);
+    ensures old(C.p)[x] == null ==> RefSetsEqual(Br, old(Br)[x := false]);
+    ensures old(C.p)[x] != null ==> RefSetsEqual(Br, (old(Br)[x := false])[old(C.p)[x] := true]);
+    // Framing conditions.
+    ensures Frame_all(
+        C.k, C.l, C.r, C.p, 
+        C.min, C.max, C.keys,
+        C.repr, C.black, C.black_height,
+        old(C.k), old(C.l), old(C.r), old(C.p), 
+        old(C.min), old(C.max), old(C.keys),
+        old(C.repr), old(C.black), old(C.black_height),
+        old(C.repr)[x], old(alloc)
+    );
+
+procedure RBTDeleteRightFixupContract(x: Ref) 
+    returns (ret: Ref, fixed: bool);
+    requires x != null;
+    requires RefSetsDisjoint(Br, (C.repr[x])[x := false]);
+    requires LC_Trans_DoubleBlack(C.k, C.l, C.r, C.p, 
+                C.min, C.max, C.keys,
+                C.repr, C.black, C.black_height, 
+                x);
+    requires (C.r[x] == null && C.l[x] != null && C.black_height[C.l[x]] == 1)
+            || (C.r[x] != null && C.l[x] != null && C.black_height[C.l[x]] == C.black_height[C.r[x]] + 1);
+    requires (C.r[x] == null || C.black[C.r[x]]);
+    requires (C.black[x] || (C.l[x] == null || C.black[C.l[x]]));
+    modifies Br, C.k, C.l, C.r, C.p, 
+                C.min, C.max, C.keys,
+                C.repr, C.black, C.black_height;
+    ensures ret != null;
+    ensures x != ret ==> (
+        C.p[x] != null
+        && C.p[x] != old(C.p)[x]
+        && (C.repr[ret])[C.p[x]]
+        && (C.l[x] != null ==> (C.repr[ret])[C.l[x]])
+        && (C.r[x] != null ==> (C.repr[ret])[C.r[x]])
+    );
+    ensures LC(C.k, C.l, C.r, C.p, 
+                C.min, C.max, C.keys,
+                C.repr, C.black, C.black_height, 
+                ret);
+    ensures C.p[ret] == null;
+    ensures KeySetsEqual(C.keys[ret], old(C.keys)[x]);
+    ensures C.min[ret] == old(C.min)[x];
+    ensures C.max[ret] == old(C.max)[x];
+    ensures RefSetsEqual(C.repr[ret], old(C.repr)[x]);
+    ensures C.black[ret] || (!C.black[ret] && !old(C.black)[x]);
+    ensures (fixed && C.black_height[ret] == old(C.black_height)[x])
+            ||  (!fixed && old(C.black)[x] && C.black_height[ret] == old(C.black_height)[x] - 1);
+    ensures old(C.p)[x] == null ==> RefSetsEqual(Br, old(Br)[x := false]);
+    ensures old(C.p)[x] != null ==> RefSetsEqual(Br, (old(Br)[x := false])[old(C.p)[x] := true]);
+    // Framing conditions.
+    ensures Frame_all(
+        C.k, C.l, C.r, C.p, 
+        C.min, C.max, C.keys,
+        C.repr, C.black, C.black_height,
+        old(C.k), old(C.l), old(C.r), old(C.p), 
+        old(C.min), old(C.max), old(C.keys),
+        old(C.repr), old(C.black), old(C.black_height),
+        old(C.repr)[x], old(alloc)
+    );
+
+procedure RBTDeleteContract(x: Ref, k: int) 
+    returns (ret: Ref, del: Ref, fixed: bool);
+    requires x != null;
+    requires RefSetsEqual(Br, EmptyRefSet);
+    requires LC(C.k, C.l, C.r, C.p, 
+                C.min, C.max, C.keys,
+                C.repr, C.black, C.black_height, 
+                x);
+    modifies Br, C.k, C.l, C.r, C.p, 
+                C.min, C.max, C.keys,
+                C.repr, C.black, C.black_height;
+    ensures x != ret && x != del ==> C.p[x] != old(C.p)[x];
+    ensures ret != del;
+    ensures !Br[x];
+    ensures (ret == null ==>
+                KeySetsEqual(old(C.keys)[x], EmptyKeySet[k := true])
+                && RefSetsEqual(old(C.repr)[x], EmptyRefSet[x := true])
+                && del != null
+                && ((fixed && !old(C.black)[x]) || (!fixed && old(C.black)[x])));
+    ensures (ret != null ==>
+                LC(C.k, C.l, C.r, C.p, 
+                    C.min, C.max, C.keys,
+                    C.repr, C.black, C.black_height, ret)
+                && (del != null ==> 
+                        C.p[ret] == null
+                        && KeySetsEqual(C.keys[ret], (old(C.keys)[x])[k := false])
+                        && (k == old(C.min)[x] ==> C.min[ret] > old(C.min)[x])
+                        && (k != old(C.min)[x] ==> C.min[ret] == old(C.min)[x])
+                        && (k == old(C.max)[x] ==> C.max[ret] < old(C.max)[x])
+                        && (k != old(C.max)[x] ==> C.max[ret] == old(C.max)[x])
+                        && RefSetsEqual(C.repr[ret], (old(C.repr)[x])[del := false])
+                        && (C.black[ret] || (!C.black[ret] && !old(C.black)[x]))
+                        && ((C.black_height[ret] == old(C.black_height)[x] && fixed)
+                            || (C.black_height[ret] == old(C.black_height)[x] - 1 && !fixed && old(C.black)[x])))
+                && (del == null ==>
+                        C.p[ret] == old(C.p)[x]
+                        && KeySetsEqual(C.keys[ret], old(C.keys)[x])
+                        && C.min[ret] == old(C.min)[x]
+                        && C.max[ret] == old(C.max)[x]
+                        && RefSetsEqual(C.repr[ret], old(C.repr)[x])
+                        && C.black[ret] == old(C.black)[x]
+                        && C.black_height[ret] == old(C.black_height)[x]));
+    ensures del != null ==> (
+        LC(C.k, C.l, C.r, C.p, 
+            C.min, C.max, C.keys,
+            C.repr, C.black, C.black_height, del)
+        && Isolated(C.k, C.l, C.r, C.p, 
+            C.min, C.max, C.keys,
+            C.repr, C.black, C.black_height, del)
+        && (old(C.keys)[x])[k]
+        && (old(C.repr)[x])[del]
+    );
+    ensures del == null || old(C.p)[x] == null ==> RefSetsEqual(Br, EmptyRefSet);
+    ensures del != null && old(C.p)[x] != null ==> RefSetsEqual(Br, EmptyRefSet[old(C.p)[x] := true]);
+    // Framing conditions.
+    ensures Frame_all(
+        C.k, C.l, C.r, C.p, 
+        C.min, C.max, C.keys,
+        C.repr, C.black, C.black_height,
+        old(C.k), old(C.l), old(C.r), old(C.p), 
+        old(C.min), old(C.max), old(C.keys),
+        old(C.repr), old(C.black), old(C.black_height),
+        old(C.repr)[x], old(alloc)
+    );
+
+// Local conditions
+function {:inline} LC_Debug(
+    k: [Ref]int, 
+    l: [Ref]Ref,
+    r: [Ref]Ref,
+    p: [Ref]Ref,
+    min: [Ref]int,
+    max: [Ref]int,
+    keys: [Ref]KeySet,
+    repr: [Ref]RefSet,
+    black: [Ref]bool,
+    black_height: [Ref]int,
+    x: Ref
+) returns (bool)
+{
+    (x != null ==> (
+        (repr[x])[x]
+        && min[x] <= k[x] 
+        && k[x] <= max[x]
+        && (p[x] != null ==>
+                !(repr[x])[p[x]]
+                && (l[p[x]] == x || r[p[x]] == x))
+        && (l[x] != null ==> 
+                (repr[x])[l[x]]
+                && !(repr[l[x]])[x]
+                && p[l[x]] == x
+                && max[l[x]] < k[x])
+        && (r[x] != null ==> 
+                (repr[x])[r[x]]
+                && !(repr[r[x]])[x]
+                && p[r[x]] == x
+                && min[r[x]] > k[x])
+        && (l[x] == null && r[x] == null ==>
+                RefSetsEqual(repr[x], EmptyRefSet[x := true])
+                && KeySetsEqual(keys[x], EmptyKeySet[k[x] := true])
+                && min[x] == k[x] 
+                && k[x] == max[x]
+                )
+        && (l[x] != null && r[x] == null ==>
+                RefSetsEqual(repr[x], (repr[l[x]])[x := true])
+                && KeySetsEqual(keys[x], (keys[l[x]])[k[x] := true])
+                && !(keys[l[x]])[k[x]]
+                && min[x] == min[l[x]] && max[x] == k[x]
+                )
+        && (l[x] == null && r[x] != null ==>
+                RefSetsEqual(repr[x], (repr[r[x]])[x := true])
+                && KeySetsEqual(keys[x], (keys[r[x]])[k[x] := true])
+                && !(keys[r[x]])[k[x]]
+                && min[x] == k[x] && max[x] == max[r[x]]
+                )
+        && (l[x] != null && r[x] != null ==>
+                RefSetsEqual(repr[x], RefSetUnionF((repr[l[x]])[x := true], repr[r[x]]))
+                && RefSetsDisjoint(repr[l[x]], repr[r[x]])
+                && KeySetsEqual(keys[x], KeySetUnionF((keys[l[x]])[k[x] := true], keys[r[x]]))
+                && KeySetsDisjoint(keys[l[x]], keys[r[x]])
+                && !(keys[l[x]])[k[x]] && !(keys[r[x]])[k[x]]
+                && min[x] == min[l[x]] && max[x] == max[r[x]]
+                )
+        // Special RBT properties
+        && (l[x] == null && r[x] == null ==>
+                black_height[x] == (if black[x] then 1 else 0))
+        && (l[x] != null && r[x] == null ==>
+                black_height[x] == (if black[x] then 1 else 0)
+                && black_height[l[x]] == 0
+                && (black[x] || black[l[x]]))
+        && (l[x] == null && r[x] != null ==>
+                black_height[x] == (if black[x] then 1 else 0)
+                && black_height[r[x]] == 0
+                && (black[x] || black[r[x]]))
+        && (l[x] != null && r[x] != null ==>
+                (black_height[l[x]] > black_height[r[x]] ==>
+                    black_height[x] == (if black[x] then black_height[l[x]] + 1 else black_height[l[x]]))
+                && (black_height[l[x]] <= black_height[r[x]] ==>
+                        black_height[x] == (if black[x] then black_height[r[x]] + 1 else black_height[r[x]]))
+                && black_height[l[x]] == black_height[r[x]]
+                && (black[x] || (black[l[x]] && black[r[x]]))
+                )
+        && black_height[x] >= 0
+    ))
+}
+
+procedure RBTDelete(x: Ref, k: int) 
+    returns (ret: Ref, del: Ref, fixed: bool)
+    requires x != null;
+    requires RefSetsEqual(Br, EmptyRefSet);
+    requires LC(C.k, C.l, C.r, C.p, 
+                C.min, C.max, C.keys,
+                C.repr, C.black, C.black_height, 
+                x);
+    modifies Br, C.k, C.l, C.r, C.p, 
+                C.min, C.max, C.keys,
+                C.repr, C.black, C.black_height;
+    ensures x != ret && x != del ==> C.p[x] != old(C.p)[x];
+    ensures ret != del;
+    ensures !Br[x];
+    ensures (ret == null ==>
+                KeySetsEqual(old(C.keys)[x], EmptyKeySet[k := true])
+                && RefSetsEqual(old(C.repr)[x], EmptyRefSet[x := true])
+                && del != null
+                && ((fixed && !old(C.black)[x]) || (!fixed && old(C.black)[x])));
+    ensures (ret != null ==>
+                LC(C.k, C.l, C.r, C.p, 
+                    C.min, C.max, C.keys,
+                    C.repr, C.black, C.black_height, ret)
+                && (del != null ==> 
+                        C.p[ret] == null
+                        && KeySetsEqual(C.keys[ret], (old(C.keys)[x])[k := false])
+                        && (k == old(C.min)[x] ==> C.min[ret] > old(C.min)[x])
+                        && (k != old(C.min)[x] ==> C.min[ret] == old(C.min)[x])
+                        && (k == old(C.max)[x] ==> C.max[ret] < old(C.max)[x])
+                        && (k != old(C.max)[x] ==> C.max[ret] == old(C.max)[x])
+                        && RefSetsEqual(C.repr[ret], (old(C.repr)[x])[del := false])
+                        && (C.black[ret] || (!C.black[ret] && !old(C.black)[x]))
+                        && ((C.black_height[ret] == old(C.black_height)[x] && fixed)
+                            || (C.black_height[ret] == old(C.black_height)[x] - 1 && !fixed && old(C.black)[x]))
+                    )
+                && (del == null ==>
+                        C.p[ret] == old(C.p)[x]
+                        && KeySetsEqual(C.keys[ret], old(C.keys)[x])
+                        && C.min[ret] == old(C.min)[x]
+                        && C.max[ret] == old(C.max)[x]
+                        && RefSetsEqual(C.repr[ret], old(C.repr)[x])
+                        && C.black[ret] == old(C.black)[x]
+                        && C.black_height[ret] == old(C.black_height)[x])
+                        );
+    ensures del != null ==> (
+        LC(C.k, C.l, C.r, C.p, 
+            C.min, C.max, C.keys,
+            C.repr, C.black, C.black_height, del)
+        && Isolated(C.k, C.l, C.r, C.p, 
+            C.min, C.max, C.keys,
+            C.repr, C.black, C.black_height, del)
+        && (old(C.keys)[x])[k]
+        && (old(C.repr)[x])[del]
+    );
+    ensures del == null || old(C.p)[x] == null ==> RefSetsEqual(Br, EmptyRefSet);
+    ensures del != null && old(C.p)[x] != null ==> RefSetsEqual(Br, EmptyRefSet[old(C.p)[x] := true]);
+    // Framing conditions.
+    ensures Frame_all(
+        C.k, C.l, C.r, C.p, 
+        C.min, C.max, C.keys,
+        C.repr, C.black, C.black_height,
+        old(C.k), old(C.l), old(C.r), old(C.p), 
+        old(C.min), old(C.max), old(C.keys),
+        old(C.repr), old(C.black), old(C.black_height),
+        old(C.repr)[x], old(alloc)
+    );
+{
+    // Local variables
+    var xl: Ref;
+    var xr: Ref;
+    var min: int;
+    var n: Ref;
+    var minnode: Ref;
+    var delnode: Ref;
+
+    // Subexpressions
+    var x_k: int; var x_black: bool;
+    var xr_black_height: int;
+    var xr_l: Ref; var xr_r: Ref;
+    var xl_black_height: int;
+    var xl_l: Ref; var xl_r: Ref;
+    var x_l: Ref; var x_r: Ref;
+    var x_l_min: int; var x_l_keys: KeySet; var x_l_repr: RefSet;
+    var x_r_max: int; var x_r_keys: KeySet; var x_r_repr: RefSet;
+    var x_black_height: int;
+
+    call InAllocParam(x);
+
+    call x_k := Get_k(x);
+    if (k == x_k) {
+        call xl := Get_l(x);
+        call xr := Get_r(x);
+
+        call IfNotBr_ThenLC(xl);
+        call IfNotBr_ThenLC(xr);
+
+        if (xl == null && xr == null) {
+            call Set_p(x, null);
+            call AssertLCAndRemove(x);
+            call x_black := Get_black(x);
+            fixed := !x_black;
+            ret := null; del := x;
+        } else if (xl == null) {
+            call Set_p(x, null);
+            call Set_l(x, null);
+            call Set_r(x, null);
+            call Set_p(xr, null);
+            call x_k := Get_k(x);
+            call Set_min(x, x_k);
+            call Set_max(x, x_k);
+            call Set_repr(x, EmptyRefSet[x := true]);
+            call Set_keys(x, EmptyKeySet[x_k := true]);
+            call xr_l := Get_l(xr);
+            call xr_r := Get_r(xr);
+            call IfNotBr_ThenLC(xr_l);
+            call IfNotBr_ThenLC(xr_r);
+            call Set_black(xr, true);
+            call xr_black_height := Get_black_height(xr);
+            call Set_black_height(xr, xr_black_height + 1);
+
+            call AssertLCAndRemove(x);
+            call AssertLCAndRemove(xr);
+
+            fixed := true;
+            ret := xr; del := x;
+        } else if (xr == null) {
+            call Set_p(x, null);
+            call Set_l(x, null);
+            call Set_r(x, null);
+            call Set_p(xl, null);
+            call x_k := Get_k(x);
+            call Set_min(x, x_k);
+            call Set_max(x, x_k);
+            call Set_repr(x, EmptyRefSet[x := true]);
+            call Set_keys(x, EmptyKeySet[x_k := true]);
+            call xl_l := Get_l(xl);
+            call xl_r := Get_r(xl);
+            call IfNotBr_ThenLC(xl_l);
+            call IfNotBr_ThenLC(xl_r);
+            call Set_black(xl, true);
+            call xl_black_height := Get_black_height(xl);
+            call Set_black_height(xl, xl_black_height + 1);
+
+            call AssertLCAndRemove(x);
+            call AssertLCAndRemove(xl);
+
+            fixed := true;
+            ret := xl; del := x;
+        } else {
+            call min := RBTFindMinContract(xr);
+
+            call n, minnode, fixed := RBTDeleteContract(xr, min);
+
+            call IfNotBr_ThenLC(xr);
+            
+            if (minnode == null) {
+                call IfNotBr_ThenLC(x);
+                ret := x;
+                del := null;
+                fixed := true;
+                return;
+            }
+
+            call Set_k(x, min);
+            call Set_p(x, null);
+            call Set_r(x, n);
+            if (n != null) {
+                call Set_p(n, x);
+            }
+            call AssertLCAndRemove(xr);
+
+            call x_l := Get_l(x);
+            call x_r := Get_r(x);
+            call x_k := Get_k(x);
+            call x_black := Get_black(x);
+            call x_black_height := Get_black_height(x);
+            if (x_l != null) {
+                call x_l_min := Get_min(x_l);
+                call x_l_keys := Get_keys(x_l);
+                call x_l_repr := Get_repr(x_l);
+            }
+            if (x_r != null) {
+                call x_r_max := Get_max(x_r);
+                call x_r_keys := Get_keys(x_r);
+                call x_r_repr := Get_repr(x_r);
+            }
+            call Set_min(x, if x_l == null then x_k else x_l_min);
+            call Set_max(x, if x_r == null then x_k else x_r_max);
+            call Set_keys(x, 
+                KeySetUnionF(
+                    (if x_l == null then EmptyKeySet else x_l_keys)[x_k := true],
+                    if x_r == null then EmptyKeySet else x_r_keys
+                )
+            );
+            call Set_repr(x, 
+                RefSetUnionF(
+                    (if x_l == null then EmptyRefSet else x_l_repr)[x := true],
+                    if x_r == null then EmptyRefSet else x_r_repr
+                )
+            );
+
+            call AssertLCAndRemove(n);
+
+            if (fixed) {
+                call AssertLCAndRemove(x);
+
+                ret := x; del := minnode;
+                fixed := true;
+            } else {
+                call ret, fixed := RBTDeleteRightFixupContract(x);
+                del := minnode;
+            }
+        }
+    } else if (k < x_k) {
+        call x_l := Get_l(x);
+        call x_r := Get_r(x);
+        call IfNotBr_ThenLC(x_l);
+        call IfNotBr_ThenLC(x_r);
+
+        if (x_l == null) {
+            ret := x;
+            del := null;
+            fixed := true;
+            return;
+        }
+
+        call n, delnode, fixed := RBTDeleteContract(x_l, k);
+
+        call x_l := Get_l(x);
+        if (x_l != null) {
+            call IfNotBr_ThenLC(x_l);
+        }
+
+        if (delnode == null) {
+            call IfNotBr_ThenLC(x);
+            ret := x;
+            del := null;
+            fixed := true;
+            return;
+        }
+
+        assume false;
+    } else {
+        assume false;
+    }
+}
